ExistentialRules/Triggers/Obsolescence.lean
@@ -8,15 +8,15 @@ module
 public import ExistentialRules.Triggers.Basic
 
 /-!
-# Obsoleteness (Conditions)
+# Obsolescence (Conditions)
 
 For the chase, we need to be able to define when a trigger should not be applied even though it might be loaded.
 In such a case (even when not loaded), we say that the trigger is "obsolete".
 We make this decision based on a given `PreTrigger` and a `FactSet`.
-Different chase variants use different notions of obsoleteness.
+Different chase variants use different notions of obsolescence.
 For example the restricted (aka. standard) chase says that a trigger is obsolete when it is satisfied.
 On the other hand, the Skolem chase says that a trigger is obsolete when its excat result is already present.
-We aim to capture both of these notions and everything in-between using a generic `ObsoletenessCondition`
+We aim to capture both of these notions and everything in-between using a generic `ObsolescenceCondition`
 that conveys the necessary properties.
 
 The condition itself is a function taking a `PreTrigger` and a `FactSet` returning a `Prop` indicating if the trigger is obsolete for the fact set or not.
@@ -27,25 +27,25 @@ Then, we require 4 conditions:
 3. If the exact trigger result already occurs in the fact set, then the trigger is obsolete.
 4. Equivalent triggers are obsolete on exactly the same fact sets.
 
-`RestrictedObsoleteness` and `SkolemObsoleteness` are the two extremes of what is allowed according to these conditions, `SkolemObsoleteness` being the most liberal and `RestrictedObsoleteness` being, quite expectedly, the most restricted.
+`RestrictedObsolescence` and `SkolemObsolescence` are the two extremes of what is allowed according to these conditions, `SkolemObsolescence` being the most liberal and `RestrictedObsolescence` being, quite expectedly, the most restricted.
 -/
 
 public section
 
-/-- `LaxObsoletenessCondition` is a more liberal version of `ObsoletenessCondition` enforcing only subset monotonicity (i.e. condition 1 above). We use such a more liberal condition for MFA later. For the most part, you can completely ignore that this exists and only consider `ObsoletenessCondition`s instead. -/
-structure LaxObsoletenessCondition (sig : Signature) [DecidableEq sig.P] [DecidableEq sig.C] [DecidableEq sig.V] where
+/-- `LaxObsolescenceCondition` is a more liberal version of `ObsolescenceCondition` enforcing only subset monotonicity (i.e. condition 1 above). We use such a more liberal condition for MFA later. For the most part, you can completely ignore that this exists and only consider `ObsolescenceCondition`s instead. -/
+structure LaxObsolescenceCondition (sig : Signature) [DecidableEq sig.P] [DecidableEq sig.C] [DecidableEq sig.V] where
   cond : PreTrigger sig -> FactSet sig -> Prop
   monotone : ∀ {trg} {A B : FactSet sig}, A ⊆ B -> cond trg A -> cond trg B
 
-/-- An `ObsoletenessCondition` is a function from `PreTrigger` and `FactSet` into `Prop` with the 4 conditions mentioned above. -/
-structure ObsoletenessCondition (sig : Signature) [DecidableEq sig.P] [DecidableEq sig.C] [DecidableEq sig.V] extends LaxObsoletenessCondition sig where
+/-- An `ObsolescenceCondition` is a function from `PreTrigger` and `FactSet` into `Prop` with the 4 conditions mentioned above. -/
+structure ObsolescenceCondition (sig : Signature) [DecidableEq sig.P] [DecidableEq sig.C] [DecidableEq sig.V] extends LaxObsolescenceCondition sig where
   cond_implies_trg_is_satisfied : cond trg fs -> trg.satisfied fs
   contains_trg_result_implies_cond : ∀ {trg : PreTrigger sig} {fs} (disj_index : Fin trg.mapped_head.length),
     ((trg.mapped_head[disj_index.val]).toSet ⊆ fs) -> cond trg fs
   preserved_under_equiv : ∀ {trg trg2 : PreTrigger sig} {fs}, trg.equiv trg2 -> (cond trg fs ↔ cond trg2 fs)
 
 instance {sig : Signature} [DecidableEq sig.P] [DecidableEq sig.C] [DecidableEq sig.V] :
-    Coe (ObsoletenessCondition sig) (LaxObsoletenessCondition sig) where
+    Coe (ObsolescenceCondition sig) (LaxObsolescenceCondition sig) where
   coe obs := { cond := obs.cond, monotone := obs.monotone }
 
 section SpecificConditions
@@ -53,12 +53,12 @@ section SpecificConditions
 /-!
 ## SpecificConditions
 
-We briefly define the `ObsoletenessCondition`s for Skolem and restricted chase to show that these indeed have the 4 necessary properties. However, most definitions are still expressed in terms of the generic `ObsoletenessCondition` so the specific ones are rarely used throughout the code; only when results indeed do not hold for the generic case but only specific obsoleteness conditions.
+We briefly define the `ObsolescenceCondition`s for Skolem and restricted chase to show that these indeed have the 4 necessary properties. However, most definitions are still expressed in terms of the generic `ObsolescenceCondition` so the specific ones are rarely used throughout the code; only when results indeed do not hold for the generic case but only specific obsolescence conditions.
 -/
 
-/-- Obsoleteness for the Skolem chase is indeed a `ObsoletenessCondition`, i.e. it has all 4 properties. According to this condition, a trigger is obsolete if its exact result, for one of the head disjuncts, already occurs in the fact set. -/
+/-- Obsolescence for the Skolem chase is indeed a `ObsolescenceCondition`, i.e. it has all 4 properties. According to this condition, a trigger is obsolete if its exact result, for one of the head disjuncts, already occurs in the fact set. -/
 @[expose]
-def SkolemObsoleteness (sig : Signature) [DecidableEq sig.P] [DecidableEq sig.C] [DecidableEq sig.V] : ObsoletenessCondition sig := {
+def SkolemObsolescence (sig : Signature) [DecidableEq sig.P] [DecidableEq sig.C] [DecidableEq sig.V] : ObsolescenceCondition sig := {
   cond := fun (trg : PreTrigger sig) (fs : FactSet sig) => ∃ i : Fin trg.mapped_head.length, (trg.mapped_head[i.val]).toSet ⊆ fs
   monotone := by
     intro trg A B A_sub_B
@@ -91,9 +91,9 @@ def SkolemObsoleteness (sig : Signature) [DecidableEq sig.P] [DecidableEq sig.C]
       exact h
 }
 
-/-- Obsoleteness for the restricted chase is indeed a `ObsoletenessCondition`, i.e. it has all 4 properties. According to this condition, a trigger is obsolete if it is satisfied. -/
+/-- Obsolescence for the restricted chase is indeed a `ObsolescenceCondition`, i.e. it has all 4 properties. According to this condition, a trigger is obsolete if it is satisfied. -/
 @[expose]
-def RestrictedObsoleteness (sig : Signature) [DecidableEq sig.P] [DecidableEq sig.C] [DecidableEq sig.V] : ObsoletenessCondition sig := {
+def RestrictedObsolescence (sig : Signature) [DecidableEq sig.P] [DecidableEq sig.C] [DecidableEq sig.V] : ObsolescenceCondition sig := {
   cond := fun (trg : PreTrigger sig) (fs : FactSet sig) => trg.satisfied fs
   monotone := by
     intro trg A B A_sub_B
@@ -125,7 +125,7 @@ section Trigger
 /-!
 ## (Proper) Triggers
 
-A `Trigger` is a `PreTrigger` that has a fixed obsoleteness condition.
+A `Trigger` is a `PreTrigger` that has a fixed obsolescence condition.
 We say that a `Trigger` is `active` if it is loaded and not obsolete.
 
 `SkolemTrigger` and `RestrictedTrigger` are just defined as examples.
@@ -133,12 +133,12 @@ We say that a `Trigger` is `active` if it is loaded and not obsolete.
 
 variable {sig : Signature} [DecidableEq sig.P] [DecidableEq sig.C] [DecidableEq sig.V]
 
-structure Trigger (obsolete : LaxObsoletenessCondition sig) extends PreTrigger sig
+structure Trigger (obsolete : LaxObsolescenceCondition sig) extends PreTrigger sig
 
-def SkolemTrigger := Trigger (SkolemObsoleteness sig : LaxObsoletenessCondition sig)
-def RestrictedTrigger := Trigger (RestrictedObsoleteness sig : LaxObsoletenessCondition sig)
+def SkolemTrigger := Trigger (SkolemObsolescence sig : LaxObsolescenceCondition sig)
+def RestrictedTrigger := Trigger (RestrictedObsolescence sig : LaxObsolescenceCondition sig)
 
-variable {obs : LaxObsoletenessCondition sig}
+variable {obs : LaxObsolescenceCondition sig}
 
 instance : CoeOut (Trigger obs) (PreTrigger sig) where
   coe trigger := { rule := trigger.rule, subs := trigger.subs }
