ExistentialRules.lean
@@ -31,6 +31,6 @@ import ExistentialRules.Terms.Basic
 import ExistentialRules.Terms.Cyclic
 import ExistentialRules.Terms.ListsOfTerms
 import ExistentialRules.Triggers.Basic
-import ExistentialRules.Triggers.Obsoleteness
+import ExistentialRules.Triggers.Obsolescence
 import ExistentialRules.Triggers.RTrigger
 
