ExistentialRules/ChaseSequence/ChaseNode.lean
@@ -20,17 +20,17 @@ It can be very useful to also keep track of the associated triggers and this is 
 public section
 
 /-- A `ChaseNode` corresponds to a chase step. It must contain a `FactSet` and optionally an `RTrigger` and a head disjunct index indicating that the current `ChaseNode` was obtained by applying the specified trigger and picking the indicated head disjunct. It is optional since the initial fact set does not result from a trigger but on all following nodes, this value will be set (and we will prove that it is). For convenience, the chase node also directly includes a proof that the result of its origin is indeed contained in its fact set. -/
-structure ChaseNode (obs : ObsoletenessCondition sig) (rules : RuleSet sig) where
+structure ChaseNode (obs : ObsolescenceCondition sig) (rules : RuleSet sig) where
   facts : FactSet sig
   -- the origin is none only for the database
-  origin : Option ((trg : RTrigger (obs : LaxObsoletenessCondition sig) rules) × Fin trg.val.mapped_head.length)
+  origin : Option ((trg : RTrigger (obs : LaxObsolescenceCondition sig) rules) × Fin trg.val.mapped_head.length)
   facts_contain_origin_result : ∀ orig ∈ origin, orig.fst.val.mapped_head[orig.snd.val].toSet ⊆ facts
 
 namespace ChaseNode
 
 /-- The `origin_result` denotes the facts that have been introduced for the chase node. That is, the mapped head index for the trigger stored in the origin field of the `ChaseNode`. -/
 @[expose]
-def origin_result {obs : ObsoletenessCondition sig} (node : ChaseNode obs rules) (isSome : node.origin.isSome) :
+def origin_result {obs : ObsolescenceCondition sig} (node : ChaseNode obs rules) (isSome : node.origin.isSome) :
     List (Fact sig) :=
   let origin := node.origin.get isSome
   origin.fst.val.mapped_head[origin.snd.val]
