ExistentialRules/ChaseSequence/Termination/ConstantMappings/InterplayWithBacktracking/BacktrackingUnderConstantMappingSubsetOfComposingWithSubs/PreGroundTerm.lean
@@ -6,7 +6,7 @@ Released under Apache 2.0 license as described in the file LICENSE.
 module
 
 public import ExistentialRules.ChaseSequence.Termination.BacktrackingOfFacts
-public import ExistentialRules.ChaseSequence.Termination.ConstantMappings.InterplayWithObsoletenessCondition
+public import ExistentialRules.ChaseSequence.Termination.ConstantMappings.InterplayWithObsolescenceCondition
 
 /-!
 # Interaction of Backtrackings and Strict Constant Mappings on PreGroundTerm
